Reimplement FramingReference with automatic framing

ulib/experimental/Steel.FramingReference.fst
@@ -34,32 +34,42 @@ let alloc x =
   r
 
 let read #a #p #v r =
-  let v' = U.raise_val v in
+  let v' = Ghost.hide (U.raise_val (Ghost.reveal v)) in
   change_slprop (pts_to r p v) (H.pts_to r p v') (fun _ -> ());
-//  Steel.FramingEffec
   let x = H.read #_ #p #v' r in
   let v':a = U.downgrade_val x in
   change_slprop (H.pts_to r p (hide x)) (pts_to r p v') (fun _ -> ());
   v'
-//  Basics.return (U.downgrade_val x)
 
 let read_refine #a #p q r =
-  Basics.h_assert (h_exists (fun (v:a) -> pts_to r p v `star` q v));
-  Basics.lift_h_exists (fun (v:a) -> pts_to r p v `star` q v);
-  Basics.h_assert (h_exists (fun (v:U.raise_t a) -> pts_to r p (U.downgrade_val v) `star` q (U.downgrade_val v)));
-  Basics.h_exists_cong (fun (v:U.raise_t a) -> pts_to r p (U.downgrade_val v) `star` q (U.downgrade_val v))
+  A.lift_h_exists_atomic (fun (v:a) -> pts_to r p v `star` q v);
+  A.h_exists_cong_atomic (fun (v:U.raise_t a) -> pts_to r p (U.downgrade_val v) `star` q (U.downgrade_val v))
                 (fun (v:U.raise_t a) -> H.pts_to r p v `star` U.lift_dom q v);
-  Basics.h_assert (h_exists (fun (v:U.raise_t a) -> H.pts_to r p v `star` U.lift_dom q v));
   let x = H.read_refine (U.lift_dom q) r in
-  Basics.h_assert (H.pts_to r p x `star` U.lift_dom q x);
-  Basics.h_assert (pts_to r p (U.downgrade_val x) `star` q (U.downgrade_val x));
-  Basics.return (U.downgrade_val x)
+  change_slprop
+    (H.pts_to r p (hide x) `star` U.lift_dom q x)
+    (pts_to r p (U.downgrade_val x) `star` q (U.downgrade_val x)) (fun _ -> ());
 
-let write r x = H.write r (U.raise_val x)
+  (U.downgrade_val x)
 
-let free x = H.free x
+let write #a #v r x =
+  let v' = Ghost.hide (U.raise_val (Ghost.reveal v)) in
+  change_slprop (pts_to r full_perm v) (H.pts_to r full_perm v') (fun _ -> ());
+  let x' = U.raise_val x in
+  H.write #_ #v' r x';
+  change_slprop (H.pts_to r full_perm (hide x')) (pts_to r full_perm x) (fun _ -> ())
 
-let share_atomic r = H.share_atomic r
+let free #a #v r =
+  let v' = Ghost.hide (U.raise_val (Ghost.reveal v)) in
+  change_slprop (pts_to r full_perm v) (H.pts_to r full_perm v') (fun _ -> ());
+  H.free #_ #v' r
+
+let share_atomic #a #uses #p #v r =
+  let v' = Ghost.hide (U.raise_val (Ghost.reveal v)) in
+  A.change_slprop (pts_to r p v) (H.pts_to r p v') (fun _ -> ());
+  H.share_atomic #_ #_ #p #v' r;
+  A.change_slprop (H.pts_to r (half_perm p) v') (pts_to r (half_perm p) v) (fun _ -> ());
+  A.change_slprop (H.pts_to r (half_perm p) v') (pts_to r (half_perm p) v) (fun _ -> ())
 
 let hide_raise_reveal (#a:Type) (v0:erased a) (v1:erased a)
   : Lemma (hide (U.raise_val (reveal v0)) == hide (U.raise_val (reveal v1)) <==>
@@ -72,8 +82,12 @@ let hide_raise_reveal (#a:Type) (v0:erased a) (v1:erased a)
             v0 == v1)
 
 let gather_atomic #a #uses #p0 #p1 #v0 #v1 r =
-  let x = H.gather_atomic r in
-  A.return_atomic x
+  let v0' = Ghost.hide (U.raise_val (Ghost.reveal v0)) in
+  let v1' = Ghost.hide (U.raise_val (Ghost.reveal v1)) in
+  A.change_slprop (pts_to r p0 v0) (H.pts_to r p0 v0') (fun _ -> ());
+  A.change_slprop (pts_to r p1 v1) (H.pts_to r p1 v1') (fun _ -> ());
+  H.gather_atomic #_ #_ #p0 #p1 #v0' #v1' r;
+  A.change_slprop (H.pts_to r (sum_perm p0 p1) v0') (pts_to r (sum_perm p0 p1) v0) (fun _ -> ())
 
 let raise_equiv (#t:Type) (x y:t)
   : Lemma (U.raise_val x == U.raise_val y <==>
@@ -121,24 +135,3 @@ let cas_action (#t:eqtype)
 
 
 let cas #t #uses r v v_old v_new = A.as_atomic_action (cas_action #t #uses r v v_old v_new)
-
-let raise_ref r p v = Basics.return r
-
-let lower_ref r p v = Basics.return r
-
-let pts_to_witinv (#a:Type u#0) (r:ref a) (p:perm)
-  : Lemma (is_witness_invariant (pts_to r p))
-  = let aux (x y : erased a) (m : mem)
-      : Lemma (requires (interp (pts_to r p x) m
-                       /\ interp (pts_to r p y) m))
-              (ensures x == y)
-      = H.pts_to_witinv r p
-    in
-    Classical.forall_intro (fun x ->
-    Classical.forall_intro (fun y ->
-    Classical.forall_intro (fun m ->
-    Classical.move_requires (aux x y) m)))
-
-let pts_to_framon (#a:Type u#0) (r:ref a) (p:perm)
-  : Lemma (is_frame_monotonic (pts_to r p))
-  = pts_to_witinv r p
